verification/MinrootCore/Code/Types.lean
@@ -23,23 +23,43 @@ inductive error.Error where
 | ZeroIterations : error.Error
 | Truncation : error.Error
 
+/-- [minroot_core::field::add_limbs::closure#3]
+    Source: 'crates/minroot-core/src/field.rs', lines 308:46-308:67 -/
+@[reducible]
+def field.add_limbs.closure_3 := Unit
+
+/-- [minroot_core::field::add_limbs::closure#2]
+    Source: 'crates/minroot-core/src/field.rs', lines 307:46-307:67 -/
+@[reducible]
+def field.add_limbs.closure_2 := Unit
+
+/-- [minroot_core::field::add_limbs::closure#1]
+    Source: 'crates/minroot-core/src/field.rs', lines 306:46-306:67 -/
+@[reducible]
+def field.add_limbs.closure_1 := Unit
+
+/-- [minroot_core::field::add_limbs::closure]
+    Source: 'crates/minroot-core/src/field.rs', lines 305:46-305:67 -/
+@[reducible]
+def field.add_limbs.closure := Unit
+
 /-- [minroot_core::field::sub_limbs::closure#3]
-    Source: 'crates/minroot-core/src/field.rs', lines 324:46-324:67 -/
+    Source: 'crates/minroot-core/src/field.rs', lines 336:46-336:67 -/
 @[reducible]
 def field.sub_limbs.closure_3 := Unit
 
 /-- [minroot_core::field::sub_limbs::closure#2]
-    Source: 'crates/minroot-core/src/field.rs', lines 323:46-323:67 -/
+    Source: 'crates/minroot-core/src/field.rs', lines 335:46-335:67 -/
 @[reducible]
 def field.sub_limbs.closure_2 := Unit
 
 /-- [minroot_core::field::sub_limbs::closure#1]
-    Source: 'crates/minroot-core/src/field.rs', lines 322:46-322:67 -/
+    Source: 'crates/minroot-core/src/field.rs', lines 334:46-334:67 -/
 @[reducible]
 def field.sub_limbs.closure_1 := Unit
 
 /-- [minroot_core::field::sub_limbs::closure]
-    Source: 'crates/minroot-core/src/field.rs', lines 321:46-321:67 -/
+    Source: 'crates/minroot-core/src/field.rs', lines 333:46-333:67 -/
 @[reducible]
 def field.sub_limbs.closure := Unit
 
